\subsubsection{Gradient}
\begin{minipage}{0.2\linewidth}
    \begin{flalign}
        &\nabla f := \left[\begin{matrix}
            f_{,1}\\
            f_{,2}\\
            \vdots\\
            f_{,n}\\
        \end{matrix}\right]&
    \end{flalign}
\end{minipage}
\hfill
\begin{minipage}{0.8\linewidth}
    \begin{itemize}
        \item Faktor-Regel: $\nabla(a \cdot g(x)) = a \cdot \nabla g(x)$
        \item Summen-Regel: $\nabla(g(x) + h(x)) = \nabla g(x) + \nabla h(x)$
        \item Linearit√§t: $\nabla(a \cdot g(x) + b \cdot h(x)) = a \cdot \nabla g(x) + b \cdot \nabla h(x)$
        \item Produkt-Regel: \\
        $\nabla (g(x) \cdot h(x)) = \nabla g(x) \cdot h(x) + g(x) \cdot \nabla h(x)$
        \item Ketten-Regel $\mathbb{R} \Rightarrow \mathbb{R}$: $\nabla f = g'(h(x^1; \cdots ; x^n)) \cdot \nabla h(x)$
        \item Ketten-Regel $\mathbb{R}^n \Rightarrow \mathbb{R}: f'(x) = \langle \nabla g(\vec{h}(x)), \vec{h}'(x) \rangle$
    \end{itemize}
\end{minipage}